theories/theories/utp_theory.thy
@@ -10,6 +10,12 @@ theory utp_theory
 imports "../alpha/utp_alpha_pred"
 begin
 
+abbreviation is_healthy :: 
+  " 'VALUE WF_ALPHA_PREDICATE 
+  \<Rightarrow> 'VALUE ALPHA_FUNCTION 
+  \<Rightarrow> bool" ("_ is _ healthy") where
+"is_healthy p H \<equiv> p = H p"
+
 definition IDEMPOTENT_OVER ::
   "'VALUE ALPHABET \<Rightarrow> 'VALUE ALPHA_FUNCTION set" where
 "IDEMPOTENT_OVER a = {f . \<forall> p \<in> WF_ALPHA_PREDICATE_OVER a . f (f p) = f p}"
@@ -33,5 +39,8 @@ definition utp_alphabets ::
 definition healthconds :: 
   "'VALUE WF_THEORY \<Rightarrow> 'VALUE ALPHA_FUNCTION set" ("\<H>") where
 "healthconds t = snd (Rep_WF_THEORY t)"
+
+definition THEORY_PRED :: "'VALUE WF_THEORY \<Rightarrow> 'VALUE WF_ALPHA_PREDICATE set" where
+"THEORY_PRED t \<equiv> {p. \<alpha> p \<in> \<A> t \<and> (\<forall> H \<in> \<H> t. p is H healthy)}"
 
 end
